MathQL/MathQL/Context.lean
@@ -6,56 +6,44 @@ namespace MathQL
 
 /-- The typing info of a domain. -/
 structure DomainTy where
+  /-- The type of id for this domain -/
+  idTy : Ty
+  /-- Available field projections with their types -/
   inputField : List (Label × Ty)
+  /-- Available field projections in the output -/
   outputField : List Label
 
 /-- A context describing which domains are available, with their typing info. -/
 abbrev DomainContext := List (DomainName × DomainTy)
 
-def DomainContext.empty : DomainContext := []
-
-def DomainContext.extend (D : DomainContext) (x : DomainName) (d : DomainTy) : DomainContext :=
-  (x, d) :: D
-
-inductive Context.Entry where
-  | const : Ty → Entry
-  | domain : DomainTy → Entry
-
 /-- Contexts. -/
 structure Context where
   domain : DomainContext
-  var : List (Ident × Context.Entry)
+  ident : List (Ident × Ty)
 
-def Context.lookupConst (Γ : Context) (x : Ident) : Option Ty := do
-  let ent ← Γ.var.lookup x
-  match ent with
-  | .const t => return t
-  | .domain _ => .none
+def Context.lookupIdent (Γ : Context) (x : Ident) : Option Ty := Γ.ident.lookup x
 
-def Context.lookupVar (Γ : Context) (x : Ident) : Option DomainTy := do
-  let ent ← Γ.var.lookup x
-  match ent with
-  | .const _ => .none
-  | .domain d => return d
+def Context.lookupDomain (Γ : Context) (d : DomainName) : Option DomainTy := Γ.domain.lookup d
 
 def Context.lookupInputField (Γ : Context) (x : Ident) (l : Label) : Option Ty := do
-  let d ← Γ.lookupVar x
-  d.inputField.lookup l
+  let t ← Γ.lookupIdent x
+  match t with
+  | .domain d =>
+    let td ← Γ.lookupDomain d
+    td.inputField.lookup l
+  | _ => none
 
 def Context.isOutputField (Γ : Context) (x : Ident) (l : Label) : Option Bool := do
-  let d ← Γ.lookupVar x
-  return (d.outputField.elem l)
+  let t ← Γ.lookupIdent x
+  match t with
+  | .domain d =>
+    let td ← Γ.lookupDomain d
+    td.outputField.elem l
+  | _ => none
 
 def Context.empty (D : DomainContext) : Context where
   domain := D
-  var := []
+  ident := []
 
-def Context.extend (Γ : Context) (x : Ident) (ent : Entry) : Context :=
-  { domain := Γ.domain, var := (x, ent) :: Γ.var }
-
-def Context.extendMany (Γ : Context) : List (Ident × DomainName) → Option Context
-| [] => return Γ
-| (x, n) :: xns => do
-  let d ← Γ.domain.lookup n
-  let Γ := Γ.extend x (.domain d)
-  Γ.extendMany xns
+def Context.extendIdent (Γ : Context) (x : Ident) (t : Ty) : Context :=
+  { domain := Γ.domain, ident := (x, t) :: Γ.ident }
