MathQL/MathQL/Expr.lean
@@ -6,18 +6,36 @@ namespace MathQL
 
 /-- Expressions -/
 inductive Expr where
+  /-- Integer literal -/
   | int : Int → Expr
+  /-- Boolean literal -/
   | bool : Bool → Expr
+  /-- String literal -/
   | str : String → Expr
-  | const : Ident → Expr
-  | field : Ident → Label → Expr
+  /-- Predefined constant -/
+  | ident : Ident → Expr
+  /-- Object ID -/
+  | id : DomainName → Expr → Expr
+  /-- Field projection -/
+  | field : DomainName → Expr → Label → Expr
+  /-- Object with the given id -/
+  | obj : DomainName → Expr → Expr
+  /-- Unary operation -/
   | unop : UnaryOp → Expr → Expr
+  /-- Binary operation -/
   | binop : BinaryOp → Expr → Expr → Expr
+  /-- Comparison -/
   | compare : ComparisonOp → Ty → Expr → Expr → Expr
+  /-- List -/
   | list : List Expr → Expr
+  /-- Tuple -/
   | tuple : List Expr → Expr
+  /-- Tuple projection -/
   | proj : Expr → Nat → Expr
+  /-- Conditional expression -/
   | ite : Expr → Expr → Expr → Expr
+  /-- Defined? -/
   | defined : Expr → Expr
+  /-- Undefined? -/
   | undefined : Expr → Expr
 deriving Repr
